finish full port of tamarack2 example
Now everything is in a single theory: tamarackTheory. The theories
tamarack, tamarackProof1, tamarackProof2, tamarackProof3 are gone.
Moreover the proofs that were present in tamarackProof1 got changed
significantly.

examples/hardware/port-full/tamarack2/tamarackScript.sml
@@ -16,6 +16,10 @@ open arithmeticTheory stringTheory
 
 val _ = new_theory "tamarack";
 
+(* ----------------------------- *)
+(* - Definitions               - *)
+(* ----------------------------- *)
+
 val _ = type_abbrev ("time",``:num``);
 val _ = type_abbrev ("wire",``:time->bool``);
 val _ = type_abbrev ("bus",``:time->num``);
@@ -135,7 +139,8 @@ val Microcode_def = Define `
           (Microcode 12 = (Cntls ("rmem","add"),  NextMpc ("jmp",14))) /\
           (Microcode 13 = (Cntls ("rmem","sub"),  NextMpc ("inc",0)) ) /\
           (Microcode 14 = (Cntls ("rbuf","wacc"), NextMpc ("jmp",10))) /\
-          (Microcode 15 = (Cntls ("none","none"), NextMpc ("jmp",0)))`;
+          (Microcode _  = (Cntls ("none","none"), NextMpc ("jmp",0)))`;
+
 
 val miw_ty = ty_antiq (hd (tl (snd (dest_type (type_of ``Microcode``)))));
 
@@ -217,6 +222,699 @@ val Behaviour_def = Define
           !t.
             (mem (t+1),pc (t+1),acc (t+1)) =
               NextState n (mem t,pc t,acc t)`;
+
+val MicroCycles_def = Define
+         `MicroCycles n (mem,pc,acc) =
+          let opc = Opc n (Inst n (mem,pc)) in
+          (if (opc = 0) then (if (acc = 0) then 5 else 6) else
+           if (opc = 1) then 4 else
+           if (opc = 2) then 8 else
+           if (opc = 3) then 8 else
+           if (opc = 4) then 6 else
+           if (opc = 5) then 6 else
+           if (opc = 6) then 6 else
+                             5)`;
+
+val REV_TimeOfCycle_def = Define `
+  (REV_TimeOfCycle 0 n mem pc acc = 0) /\
+  (REV_TimeOfCycle (SUC t) n mem pc acc =
+     let prev = (REV_TimeOfCycle t n mem pc acc) in
+     (prev + (MicroCycles n (mem prev,pc prev,acc prev))))`;
+
+val TimeOfCycle_def = Define `
+  TimeOfCycle n (mem,pc,acc) t = REV_TimeOfCycle t n mem pc acc`;
+
+
+
+(* --------------------------- *)
+(* - Proofs 1                - *)
+(* --------------------------- *)
+
+(* Evaluation theorem.
+   One can first evaluate via e.g.
+
+   LIST_CONJ (map (CONV_RULE (RHS_CONV EVAL)) (BODY_CONJUNCTS Microcode_def))
+
+   and then copy the result, massage it a bit and finally state it
+   explicitly. That way one can increase rebustness. *)
+val Microcode_EVALS = store_thm ("Microcode_EVALS",``
+      (Microcode 0 = ((F,F,T,F,T,F,F,F,F,F,F,F,F),(F,F),0)) /\
+      (Microcode 1 = ((F,T,F,F,F,F,F,T,F,F,F,F,F),(F,F),0)) /\
+      (Microcode 2 = ((F,F,T,F,F,F,F,F,T,F,F,F,F),(T,F),0)) /\
+      (Microcode 3 = ((F,F,F,F,F,F,F,F,F,F,F,F,F),(F,T),10)) /\
+      (Microcode 4 = ((F,F,F,T,F,F,F,F,T,F,F,F,F),(T,T),0)) /\
+      (Microcode 5 = ((F,F,F,F,F,F,T,F,F,T,F,F,F),(T,T),12)) /\
+      (Microcode 6 = ((F,F,F,F,F,F,T,F,F,T,F,F,F),(T,T),13)) /\
+      (Microcode 7 = ((F,T,F,F,F,T,F,F,F,F,F,F,F),(T,T),10)) /\
+      (Microcode 8 = ((T,F,F,F,F,F,T,F,F,F,F,F,F),(T,T),10)) /\
+      (Microcode 9 = ((F,F,F,F,F,F,F,F,F,F,F,F,F),(F,F),0)) /\
+      (Microcode 10 = ((F,F,F,F,T,F,F,F,F,F,F,T,F),(F,F),0)) /\
+      (Microcode 11 = ((F,F,F,T,F,F,F,F,F,F,F,F,T),(T,T),0)) /\
+      (Microcode 12 = ((F,T,F,F,F,F,F,F,F,F,F,F,F),(T,T),14)) /\
+      (Microcode 13 = ((F,T,F,F,F,F,F,F,F,F,T,F,F),(F,F),0)) /\
+      (Microcode 14 = ((F,F,F,F,F,T,F,F,F,F,F,F,T),(T,T),10)) /\
+      (Microcode 15 = ((F,F,F,F,F,F,F,F,F,F,F,F,F),(T,T),0)) /\
+      (!v. ((v <> 0) /\ (v <> 1) /\ (v <> 2) /\ (v <> 3) /\ (v <> 4) /\
+            (v <> 5) /\ (v <> 6) /\ (v <> 7) /\ (v <> 8) /\ (v <> 9) /\
+            (v <> 10) /\ (v <> 11) /\ (v <> 12) /\ (v <> 13) /\ (v <> 14)) ==>
+         (Microcode v = ((F,F,F,F,F,F,F,F,F,F,F,F,F),(T,T),0)))``,
+EVAL_TAC >> SIMP_TAC std_ss []);
+
+
+(* The following tactics correspond to the sequence of steps which take
+   place when a microinstruction is executed:
+
+   tac1 - produce microcode ROM output;
+   tac2 - generate next mpc state;
+   tac3 - generate next data path state.
+ *)
+
+val tac1 : tactic =
+  PURE_REWRITE_TAC [Tamarack_def, CntlUnit_def, ROM_def] THEN
+  REPEAT STRIP_TAC THEN
+  IMP_RES_THEN (MP_TAC o (SPEC ``t:time``)) (fst (EQ_IMP_RULE (SPEC_ALL Decoder_def))) THEN
+  ASM_REWRITE_TAC [Microcode_EVALS, pairTheory.PAIR_EQ] THEN
+  STRIP_TAC
+
+val tac2 : tactic =
+  IMP_RES_THEN MP_TAC (fst (EQ_IMP_RULE (SPEC_ALL MpcUnit_def))) THEN
+  PURE_ONCE_REWRITE_TAC [AND_def,OR_def,MUX_def,HWC_def,ADDER_def,DEL_def] THEN
+  DISCH_THEN ((REPEAT_TCL CHOOSE_THEN) (fn thm => REWRITE_TAC [thm])) THEN
+  ASM_REWRITE_TAC [];
+
+val tac3 : tactic =
+  IMP_RES_THEN MP_TAC (fst (EQ_IMP_RULE (SPEC_ALL DataPath_def))) THEN
+  PURE_ONCE_REWRITE_TAC [CheckCntls_def,MEM_def,REG_def,BITS_def,TNZ_def,ALU_def,PWR_def,GND_def] THEN
+  DISCH_THEN ((REPEAT_TCL CHOOSE_THEN) MP_TAC) THEN
+  DISCH_THEN (MP_TAC o LIST_CONJ o (map (SPEC ``t:time``)) o CONJUNCTS) THEN
+  ASM_REWRITE_TAC [pairTheory.PAIR_EQ] THEN
+  DISCH_THEN (fn thm => MP_TAC (REWRITE_RULE [CONJUNCT1 thm] (CONJUNCT2 thm))) THEN
+  STRIP_TAC THEN
+  ASM_REWRITE_TAC [];
+
+(* Combined Tactic *)
+val MPC_n_TAC =
+  tac1 >> tac2 >> tac3 >>
+  SIMP_TAC arith_ss [ADDn_def]
+
+val MPC_0_THM = store_thm ("MPC_0_THM",
+``!n mpc mem mar pc acc ir arg buf.
+  Tamarack n (mpc,mem,mar,pc,acc,ir,arg,buf)
+  ==>
+  !t.
+    (mpc t = 0) ==>
+    ((mpc (t+1),mem (t+1),mar (t+1),pc (t+1),acc (t+1)) =
+     (1,mem t,pc t,pc t,acc t))``,
+
+  MPC_n_TAC
+);
+
+
+val MPC_1_THM = store_thm ("MPC_1_THM",
+``!n mpc mem mar pc acc ir arg buf.
+  Tamarack n (mpc,mem,mar,pc,acc,ir,arg,buf)
+  ==>
+  !t.
+    (mpc t = 1) ==>
+    ((mpc (t+1),mem (t+1),pc (t+1),acc (t+1),ir (t+1)) =
+     (2,mem t,pc t,acc t,mem t (Bits (0,n) (mar t))))``,
+
+  MPC_n_TAC
+);
+
+
+val MPC_2_THM = store_thm ("MPC_2_THM",
+``!n mpc mem mar pc acc ir arg buf.
+  Tamarack n (mpc,mem,mar,pc,acc,ir,arg,buf)
+  ==>
+  !t.
+    (mpc t = 2) ==>
+    ((mpc (t+1),mem (t+1),mar (t+1),pc (t+1),acc (t+1),ir (t+1)) =
+     ((Bits (n,3) (ir t)) + 3,mem t,ir t,pc t,acc t,ir t))``,
+
+  MPC_n_TAC >>
+  `Bits (n,3) (ir t) < 8` by SIMP_TAC arith_ss [Bits_def] >>
+  DECIDE_TAC
+);
+
+
+
+val MPC_3_THM = store_thm ("MPC_3_THM",
+``!n mpc mem mar pc acc ir arg buf.
+  Tamarack n (mpc,mem,mar,pc,acc,ir,arg,buf)
+  ==>
+  !t.
+    (mpc t = 3) ==>
+    ((mpc (t+1),mem (t+1),pc (t+1),acc (t+1),ir (t+1)) =
+     (((if ((acc t) = 0) then 4 else 10),mem t,pc t,acc t,ir t)))``,
+  MPC_n_TAC
+);
+
+
+val MPC_4_THM = store_thm ("MPC_4_THM",
+``!n mpc mem mar pc acc ir arg buf.
+  Tamarack n (mpc,mem,mar,pc,acc,ir,arg,buf)
+  ==>
+  !t.
+    (mpc t = 4) ==>
+    ((mpc (t+1),mem (t+1),pc (t+1),acc (t+1)) =
+     (0,mem t,ir t,acc t))``,
+
+  MPC_n_TAC
+);
+
+
+val MPC_5_THM = store_thm ("MPC_5_THM",
+``!n mpc mem mar pc acc ir arg buf.
+  Tamarack n (mpc,mem,mar,pc,acc,ir,arg,buf)
+  ==>
+  !t.
+    (mpc t = 5) ==>
+    ((mpc (t+1),mem (t+1),mar (t+1),pc (t+1),acc (t+1),arg (t+1)) =
+     (12,mem t,mar t,pc t,acc t,acc t))``,
+
+  MPC_n_TAC
+);
+
+
+val MPC_6_THM = store_thm ("MPC_6_THM",
+``!n mpc mem mar pc acc ir arg buf.
+  Tamarack n (mpc,mem,mar,pc,acc,ir,arg,buf)
+  ==>
+  !t.
+    (mpc t = 6) ==>
+    ((mpc (t+1),mem (t+1),mar (t+1),pc (t+1),acc (t+1),arg (t+1)) =
+     (13,mem t,mar t,pc t,acc t,acc t))``,
+
+  MPC_n_TAC
+);
+
+
+val MPC_7_THM = store_thm ("MPC_7_THM",
+``!n mpc mem mar pc acc ir arg buf.
+  Tamarack n (mpc,mem,mar,pc,acc,ir,arg,buf)
+  ==>
+  !t.
+    (mpc t = 7) ==>
+    ((mpc (t+1),mem (t+1),pc (t+1),acc (t+1)) =
+     (10,mem t,pc t,mem t (Bits (0,n) (mar t))))``,
+
+  MPC_n_TAC
+);
+
+
+val MPC_8_THM = store_thm ("MPC_8_THM",
+``!n mpc mem mar pc acc ir arg buf.
+  Tamarack n (mpc,mem,mar,pc,acc,ir,arg,buf)
+  ==>
+  !t.
+    (mpc t = 8) ==>
+    ((mpc (t+1),mem (t+1),pc (t+1),acc (t+1)) =
+     (10,Update (mem t,Bits (0,n) (mar t),acc t),pc t,acc t))``,
+
+  MPC_n_TAC
+);
+
+
+val MPC_9_THM = store_thm ("MPC_9_THM",
+``!n mpc mem mar pc acc ir arg buf.
+  Tamarack n (mpc,mem,mar,pc,acc,ir,arg,buf)
+  ==>
+  !t.
+    (mpc t = 9) ==>
+    ((mpc (t+1),mem (t+1),pc (t+1),acc (t+1)) =
+     (10,mem t,pc t,acc t))``,
+
+  MPC_n_TAC
+);
+
+
+
+val MPC_10_THM = store_thm ("MPC_10_THM",
+``!n mpc mem mar pc acc ir arg buf.
+  Tamarack n (mpc,mem,mar,pc,acc,ir,arg,buf)
+  ==>
+  !t.
+    (mpc t = 10) ==>
+    ((mpc (t+1),mem (t+1),pc (t+1),acc (t+1),buf (t+1)) =
+     (11,mem t,pc t,acc t,INCn (n+3) (pc t)))``,
+
+  MPC_n_TAC
+);
+
+
+val MPC_11_THM = store_thm ("MPC_11_THM",
+``!n mpc mem mar pc acc ir arg buf.
+  Tamarack n (mpc,mem,mar,pc,acc,ir,arg,buf)
+  ==>
+  !t.
+    (mpc t = 11) ==>
+    ((mpc (t+1),mem (t+1),pc (t+1),acc (t+1)) =
+     (0,mem t,buf t,acc t))``,
+
+  MPC_n_TAC
+);
+
+
+val MPC_12_THM = store_thm ("MPC_12_THM",
+``!n mpc mem mar pc acc ir arg buf.
+  Tamarack n (mpc,mem,mar,pc,acc,ir,arg,buf)
+  ==>
+  !t.
+    (mpc t = 12) ==>
+    ((mpc (t+1),mem (t+1),pc (t+1),acc (t+1),buf (t+1)) =
+     (14,mem t,pc t,acc t,
+      ADDn (n+3) (arg t,mem t (Bits (0,n) (mar t)))))``,
+
+  MPC_n_TAC
+);
+
+
+val MPC_13_THM = store_thm ("MPC_13_THM",
+``!n mpc mem mar pc acc ir arg buf.
+  Tamarack n (mpc,mem,mar,pc,acc,ir,arg,buf)
+  ==>
+  !t.
+    (mpc t = 13) ==>
+    ((mpc (t+1),mem (t+1),pc (t+1),acc (t+1),buf (t+1)) =
+     (14,mem t,pc t,acc t,
+      SUBn (n+3) (arg t,mem t (Bits (0,n) (mar t)))))``,
+
+  MPC_n_TAC);
+
+
+val MPC_14_THM = store_thm ("MPC_14_THM",
+``!n mpc mem mar pc acc ir arg buf.
+  Tamarack n (mpc,mem,mar,pc,acc,ir,arg,buf)
+  ==>
+  !t.
+    (mpc t = 14) ==>
+    ((mpc (t+1),mem (t+1),pc (t+1),acc (t+1)) =
+     (10,mem t,pc t,buf t))``,
+
+  MPC_n_TAC);
+
+
+val MPC_15_THM = store_thm ("MPC_15_THM",
+``!n mpc mem mar pc acc ir arg buf.
+  Tamarack n (mpc,mem,mar,pc,acc,ir,arg,buf)
+  ==>
+  !t.
+    (mpc t = 15) ==>
+    ((mpc (t+1),mem (t+1),pc (t+1),acc (t+1)) =
+     (0,mem t,pc t,acc t))``,
+
+  MPC_n_TAC);
+
+
+(* Nowadays, we have much more computational power at our hands. We
+   can therefore prove a stronger version of theorems MPC_0_THM - MPC_15_THM
+   via brute force. The main idea is using Skolemization in reverse.
+   Apart from that, it is unfolding and a little bit of simple reordering. *)
+
+val Tamarack_EVAL_THM = store_thm ("Tamarack_EVAL_THM",
+   ``!n mpc mem mar pc acc ir arg buf.
+          Tamarack n (mpc,mem,mar,pc,acc,ir,arg,buf) <=>
+          !t.
+              if mpc t = 0 then
+                (mpc (t + 1) = 1) /\ (mem (t + 1) = mem t) /\
+                (pc (t + 1) = pc t) /\ (mar (t + 1) = pc t) /\
+                (acc (t + 1) = acc t) /\ (ir (t + 1) = ir t) /\
+                (arg (t + 1) = arg t) /\
+                (buf (t + 1) = ADDn (n + 3) (arg t,mar (t + 1)))
+              else if mpc t = 1 then
+                (mpc (t + 1) = 2) /\ (mem (t + 1) = mem t) /\
+                (mar (t + 1) = mar t) /\ (pc (t + 1) = pc t) /\
+                (acc (t + 1) = acc t) /\
+                (ir (t + 1) = mem t (Bits (0,n) (mar t))) /\
+                (arg (t + 1) = arg t) /\
+                (buf (t + 1) =
+                 ADDn (n + 3) (arg t,mem t (Bits (0,n) (mar t))))
+              else if mpc t = 2 then
+                (mpc (t + 1) = (Bits (n,3) (ir t) + 3)) /\
+                (mem (t + 1) = mem t) /\ (pc (t + 1) = pc t) /\
+                (acc (t + 1) = acc t) /\ (ir (t + 1) = ir t) /\
+                (mar (t + 1) = ir t) /\ (arg (t + 1) = arg t) /\
+                (buf (t + 1) = ADDn (n + 3) (arg t,mar (t + 1)))
+              else if mpc t = 3 then
+                (mpc (t + 1) = if acc t = 0 then 4 else 10) /\
+                (mem (t + 1) = mem t) /\ (mar (t + 1) = mar t) /\
+                (pc (t + 1) = pc t) /\ (acc (t + 1) = acc t) /\
+                (ir (t + 1) = ir t) /\ (arg (t + 1) = arg t) /\
+                ?bus. buf (t + 1) = ADDn (n + 3) (arg t,bus)
+              else if mpc t = 4 then
+                (mpc (t + 1) = 0) /\ (mem (t + 1) = mem t) /\
+                (mar (t + 1) = mar t) /\ (acc (t + 1) = acc t) /\
+                (ir (t + 1) = ir t) /\ (pc (t + 1) = ir t) /\
+                (arg (t + 1) = arg t) /\
+                (buf (t + 1) = ADDn (n + 3) (arg t,pc (t + 1)))
+              else if mpc t = 5 then
+                (mpc (t + 1) = 12) /\ (mem (t + 1) = mem t) /\
+                (mar (t + 1) = mar t) /\ (pc (t + 1) = pc t) /\
+                (acc (t + 1) = acc t) /\ (ir (t + 1) = ir t) /\
+                (arg (t + 1) = acc t) /\
+                (buf (t + 1) = ADDn (n + 3) (arg t,acc t))
+              else if mpc t = 6 then
+                (mpc (t + 1) = 13) /\ (mem (t + 1) = mem t) /\
+                (mar (t + 1) = mar t) /\ (pc (t + 1) = pc t) /\
+                (acc (t + 1) = acc t) /\ (ir (t + 1) = ir t) /\
+                (arg (t + 1) = acc t) /\
+                (buf (t + 1) = ADDn (n + 3) (arg t,acc t))
+              else if mpc t = 7 then
+                (mpc (t + 1) = 10) /\ (mem (t + 1) = mem t) /\
+                (mar (t + 1) = mar t) /\ (pc (t + 1) = pc t) /\
+                (acc (t + 1) = mem t (Bits (0,n) (mar t))) /\
+                (ir (t + 1) = ir t) /\ (arg (t + 1) = arg t) /\
+                (buf (t + 1) =
+                 ADDn (n + 3) (arg t,mem t (Bits (0,n) (mar t))))
+              else if mpc t = 8 then
+                (mpc (t + 1) = 10) /\
+                (mem (t + 1) = (Bits (0,n) (mar t) =+ acc t) (mem t)) /\
+                (mar (t + 1) = mar t) /\ (pc (t + 1) = pc t) /\
+                (acc (t + 1) = acc t) /\ (ir (t + 1) = ir t) /\
+                (arg (t + 1) = arg t) /\
+                (buf (t + 1) = ADDn (n + 3) (arg t,acc t))
+              else if mpc t = 9 then
+                (mpc (t + 1) = 10) /\ (mem (t + 1) = mem t) /\
+                (mar (t + 1) = mar t) /\ (pc (t + 1) = pc t) /\
+                (acc (t + 1) = acc t) /\ (ir (t + 1) = ir t) /\
+                (arg (t + 1) = arg t) /\
+                ?bus. buf (t + 1) = ADDn (n + 3) (arg t, bus)
+              else if mpc t = 10 then
+                (mpc (t + 1) = 11) /\ (mem (t + 1) = mem t) /\
+                (mar (t + 1) = mar t) /\ (pc (t + 1) = pc t) /\
+                (acc (t + 1) = acc t) /\ (ir (t + 1) = ir t) /\
+                (arg (t + 1) = arg t) /\ (buf (t + 1) = INCn (n + 3) (pc t))
+              else if mpc t = 11 then
+                (mpc (t + 1) = 0) /\ (mem (t + 1) = mem t) /\
+                (mar (t + 1) = mar t) /\ (acc (t + 1) = acc t) /\
+                (ir (t + 1) = ir t) /\ (arg (t + 1) = arg t) /\
+                (buf (t + 1) = ADDn (n + 3) (arg t,pc (t + 1))) /\
+                (pc (t + 1) = buf t)
+              else if mpc t = 12 then
+                (mpc (t + 1) = 14) /\ (mem (t + 1) = mem t) /\
+                (mar (t + 1) = mar t) /\ (pc (t + 1) = pc t) /\
+                (acc (t + 1) = acc t) /\ (ir (t + 1) = ir t) /\
+                (arg (t + 1) = arg t) /\
+                (buf (t + 1) =
+                 ADDn (n + 3) (arg t,mem t (Bits (0,n) (mar t))))
+              else if mpc t = 13 then
+                (mpc (t + 1) = 14) /\ (mem (t + 1) = mem t) /\
+                (mar (t + 1) = mar t) /\ (pc (t + 1) = pc t) /\
+                (acc (t + 1) = acc t) /\ (ir (t + 1) = ir t) /\
+                (arg (t + 1) = arg t) /\
+                (buf (t + 1) =
+                 SUBn (n + 3) (arg t,mem t (Bits (0,n) (mar t))))
+              else if mpc t = 14 then
+                (mpc (t + 1) = 10) /\ (mem (t + 1) = mem t) /\
+                (mar (t + 1) = mar t) /\ (pc (t + 1) = pc t) /\
+                (ir (t + 1) = ir t) /\ (arg (t + 1) = arg t) /\
+                (buf (t + 1) = ADDn (n + 3) (arg t,acc (t + 1))) /\
+                (acc (t + 1) = buf t)
+              else
+                (mpc (t + 1) = 0) /\ (mem (t + 1) = mem t) /\
+                (mar (t + 1) = mar t) /\ (pc (t + 1) = pc t) /\
+                (acc (t + 1) = acc t) /\ (ir (t + 1) = ir t) /\
+                (arg (t + 1) = arg t) /\
+                ?bus. buf (t + 1) = ADDn (n + 3) (arg t,bus)``,
+
+REPEAT STRIP_TAC >>
+SIMP_TAC std_ss [Tamarack_def, CntlUnit_def,
+  ROM_def, Decoder_def, MpcUnit_def, DataPath_def,
+  AND_def, OR_def, MUX_def, HWC_def, MEM_def, ALU_def, REG_def,
+  BITS_def, DEL_def, CheckCntls_def,
+  ADDER_def, PWR_def, GND_def, TNZ_def,
+  GSYM FORALL_AND_THM, PULL_EXISTS] >>
+SIMP_TAC std_ss [GSYM SKOLEM_THM] >>
+ConseqConv.CONSEQ_CONV_TAC (K ConseqConv.FORALL_EQ___CONSEQ_CONV) >>
+SIMP_TAC pure_ss [prove (``(X:'a = if c then x1 else x2) <=> (if c then (X = x1) else (X = x2))``,
+                   Cases_on `c` >> REWRITE_TAC[])] >>
+SIMP_TAC (std_ss++boolSimps.EQUIV_EXTRACT_ss) [Microcode_EVALS, ADDn_def,
+  Update_def, GSYM PULL_EXISTS] >>
+`!n m. (Bits (n,3) m + 3) < 16` by (
+  REPEAT GEN_TAC >>
+  `Bits (n, 3) m < 8` by SIMP_TAC arith_ss [Bits_def] >>
+  DECIDE_TAC
+) >>
+ASM_SIMP_TAC (arith_ss++boolSimps.LIFT_COND_ss) []);
+
+
+
+(* --------------------------- *)
+(* - Proofs 2                - *)
+(* --------------------------- *)
+
+fun EXEC_MPC_TAC tm =
+  Q.PAT_ASSUM `Tamarack _ _` (fn thm => let
+    val thm0 = CONV_RULE (REWR_CONV Tamarack_EVAL_THM) thm
+    val thm1 = SPEC tm thm0
+  in MP_TAC thm1 end) >>
+  SUBST1_TAC (SIMP_CONV arith_ss [] ``^tm + 1``) >>
+  ASM_SIMP_TAC std_ss [ADDn_def, Bits_def] >>
+  STRIP_TAC
+
+fun EXEC_MPC_TACn n = let
+  fun mk_tm n = let val m = numLib.term_of_int n in ``(t:time) + ^m`` end
+  val ns = Lib.for 0 (n-1) mk_tm
+in
+  EVERY (map EXEC_MPC_TAC ns)
+end
+
+fun EXEC_INST_FETCH_TAC n =
+   SIMP_TAC arith_ss [Opc_def,Inst_def] >>
+   REPEAT (FIRST [GEN_TAC,DISCH_THEN STRIP_ASSUME_TAC]) >>
+   EXEC_MPC_TACn n
+
+
+val JZR_T_INST_THM = store_thm ("JZR_T_INST_THM",
+``!n mpc mem mar pc acc ir arg buf.
+  Tamarack n (mpc,mem,mar,pc,acc,ir,arg,buf)
+  ==>
+  !t.
+    (mpc t = 0) /\
+    (Opc n (Inst n (mem t,pc t)) = 0) /\
+    (acc t = 0)
+    ==>
+    (mpc (t+5) = 0) /\
+    ((mem (t+5),pc (t+5),acc (t+5)) =
+      NextState n (mem t,pc t,acc t))``,
+
+EXEC_INST_FETCH_TAC 5 >>
+ASM_SIMP_TAC std_ss [NextState_def, LET_DEF, Inst_def, Opc_def]);
+
+
+val JZR_F_INST_THM = store_thm ("JZR_F_INST_THM",
+``!n mpc mem mar pc acc ir arg buf.
+  Tamarack n (mpc,mem,mar,pc,acc,ir,arg,buf)
+  ==>
+  !t.
+    (mpc t = 0) /\
+    (Opc n (Inst n (mem t,pc t)) = 0) /\
+    ~(acc t = 0)
+    ==>
+    (mpc (t+6) = 0) /\
+    ((mem (t+6),pc (t+6),acc (t+6)) =
+      NextState n (mem t,pc t,acc t))``,
+
+EXEC_INST_FETCH_TAC 6 >>
+ASM_SIMP_TAC std_ss [NextState_def, LET_DEF, Inst_def, Opc_def]);
+
+
+val JMP_INST_THM = store_thm ("JMP_INST_THM",
+``!n mpc mem mar pc acc ir arg buf.
+  Tamarack n (mpc,mem,mar,pc,acc,ir,arg,buf)
+  ==>
+  !t.
+    (mpc t = 0) /\
+    (Opc n (Inst n (mem t,pc t)) = 1)
+    ==>
+    (mpc (t+4) = 0) /\
+    ((mem (t+4),pc (t+4),acc (t+4)) =
+      NextState n (mem t,pc t,acc t))``,
+
+EXEC_INST_FETCH_TAC 4 >>
+ASM_SIMP_TAC std_ss [NextState_def, LET_DEF, Inst_def, Opc_def]);
+
+
+val ADD_INST_THM = store_thm ("ADD_INST_THM",
+``!n mpc mem mar pc acc ir arg buf.
+  Tamarack n (mpc,mem,mar,pc,acc,ir,arg,buf)
+  ==>
+  !t.
+    (mpc t = 0) /\
+    (Opc n (Inst n (mem t,pc t)) = 2)
+    ==>
+    (mpc (t+8) = 0) /\
+    ((mem (t+8),pc (t+8),acc (t+8)) =
+      NextState n (mem t,pc t,acc t))``,
+
+EXEC_INST_FETCH_TAC 8 >>
+ASM_SIMP_TAC std_ss [NextState_def, LET_DEF, Inst_def, Opc_def,
+  ADDn_def, Addr_def]);
+
+
+val SUB_INST_THM = store_thm ("ADD_INST_THM",
+``!n mpc mem mar pc acc ir arg buf.
+  Tamarack n (mpc,mem,mar,pc,acc,ir,arg,buf)
+  ==>
+  !t.
+    (mpc t = 0) /\
+    (Opc n (Inst n (mem t,pc t)) = 3)
+    ==>
+    (mpc (t+8) = 0) /\
+    ((mem (t+8),pc (t+8),acc (t+8)) =
+      NextState n (mem t,pc t,acc t))``,
+
+EXEC_INST_FETCH_TAC 8 >>
+ASM_SIMP_TAC std_ss [NextState_def, LET_DEF, Inst_def, Opc_def,
+  ADDn_def, Addr_def]);
+
+
+val LD_INST_THM = store_thm ("LD_INST_THM",
+``!n mpc mem mar pc acc ir arg buf.
+  Tamarack n (mpc,mem,mar,pc,acc,ir,arg,buf)
+  ==>
+  !t.
+    (mpc t = 0) /\
+    (Opc n (Inst n (mem t,pc t)) = 4)
+    ==>
+    (mpc (t+6) = 0) /\
+    ((mem (t+6),pc (t+6),acc (t+6)) =
+      NextState n (mem t,pc t,acc t))``,
+
+EXEC_INST_FETCH_TAC 6 >>
+ASM_SIMP_TAC std_ss [NextState_def, LET_DEF, Inst_def, Opc_def,
+  ADDn_def, Update_def, Addr_def]);
+
+
+val ST_INST_THM = store_thm ("ST_INST_THM",
+``!n mpc mem mar pc acc ir arg buf.
+  Tamarack n (mpc,mem,mar,pc,acc,ir,arg,buf)
+  ==>
+  !t.
+    (mpc t = 0) /\
+    (Opc n (Inst n (mem t,pc t)) = 5)
+    ==>
+    (mpc (t+6) = 0) /\
+    ((mem (t+6),pc (t+6),acc (t+6)) =
+      NextState n (mem t,pc t,acc t))``,
+
+EXEC_INST_FETCH_TAC 6 >>
+ASM_SIMP_TAC std_ss [NextState_def, LET_DEF, Inst_def, Opc_def,
+  ADDn_def, Update_def, Addr_def]);
+
+
+val NOP1_INST_THM = store_thm ("NOP1_INST_THM",
+``!n mpc mem mar pc acc ir arg buf.
+  Tamarack n (mpc,mem,mar,pc,acc,ir,arg,buf)
+  ==>
+  !t.
+    (mpc t = 0) /\
+    (Opc n (Inst n (mem t,pc t)) = 6)
+    ==>
+    (mpc (t+6) = 0) /\
+    ((mem (t+6),pc (t+6),acc (t+6)) =
+      NextState n (mem t,pc t,acc t))``,
+
+EXEC_INST_FETCH_TAC 6 >>
+ASM_SIMP_TAC std_ss [NextState_def, LET_DEF, Inst_def, Opc_def,
+  ADDn_def, Update_def, Addr_def]);
+
+
+val NOP2_INST_THM = store_thm ("NOP2_INST_THM",
+``!n mpc mem mar pc acc ir arg buf.
+  Tamarack n (mpc,mem,mar,pc,acc,ir,arg,buf)
+  ==>
+  !t.
+    (mpc t = 0) /\
+    (Opc n (Inst n (mem t,pc t)) = 7)
+    ==>
+    (mpc (t+5) = 0) /\
+    ((mem (t+5),pc (t+5),acc (t+5)) =
+      NextState n (mem t,pc t,acc t))``,
+
+EXEC_INST_FETCH_TAC 5 >>
+ASM_SIMP_TAC std_ss [NextState_def, LET_DEF, Inst_def, Opc_def,
+  ADDn_def, Update_def, Addr_def]);
+
+
+(* --------------------------- *)
+(* - Proofs 3                - *)
+(* --------------------------- *)
+
+val MicroCycles_def = Define `MicroCycles n (mem,pc,acc) =
+  let opc = Opc n (Inst n (mem,pc)) in
+  (if (opc = 0) then (if (acc = 0) then 5 else 6) else
+   if (opc = 1) then 4 else
+   if (opc = 2) then 8 else
+   if (opc = 3) then 8 else
+   if (opc = 4) then 6 else
+   if (opc = 5) then 6 else
+   if (opc = 6) then 6 else
+                     5)`;
+
+val TimeOfCycle_def = Define `
+  (TimeOfCycle n (mem,pc,acc) 0 = 0) /\
+  (TimeOfCycle n (mem,pc,acc) (SUC t) =
+     let prev = TimeOfCycle n (mem, pc, acc) t in
+     (prev + (MicroCycles n (mem prev,pc prev,acc prev))))`;
+
+
+val EVERY_INST_THM = store_thm ("EVERY_INST_THM",
+``!n mpc mem mar pc acc ir arg buf.
+  Tamarack n (mpc,mem,mar,pc,acc,ir,arg,buf)
+  ==>
+  !t.
+    (mpc t = 0)
+    ==>
+    let m = MicroCycles n (mem t,pc t,acc t) in
+    ((mpc (t+m) = 0) /\
+     ((mem (t+m),pc (t+m),acc (t+m)) =
+      NextState n (mem t,pc t,acc t)))``,
+
+REPEAT STRIP_TAC THEN
+Q.ABBREV_TAC `opc = Opc n (Inst n (mem t,pc t))` >>
+ASM_SIMP_TAC std_ss [MicroCycles_def, LET_DEF] >>
+
+`(opc = 0) \/ (opc = 1) \/ (opc = 2) \/ (opc = 3) \/
+ (opc = 4) \/ (opc = 5) \/ (opc = 6) \/ (opc = 7)` by (
+   `opc < 8` suffices_by DECIDE_TAC >>
+   Q.UNABBREV_TAC `opc` >>
+   SIMP_TAC arith_ss [Opc_def]
+) >> ASM_SIMP_TAC std_ss [] >| [
+  PROVE_TAC [JZR_T_INST_THM, JZR_F_INST_THM],
+  PROVE_TAC [JMP_INST_THM],
+  PROVE_TAC [ADD_INST_THM],
+  PROVE_TAC [SUB_INST_THM],
+  PROVE_TAC [LD_INST_THM],
+  PROVE_TAC [ST_INST_THM],
+  PROVE_TAC [NOP1_INST_THM],
+  PROVE_TAC [NOP2_INST_THM]
+]);
+
+val ALWAYS_MPC_0_THM = store_thm ("ALWAYS_MPC_0_THM",
+``!n mpc mem mar pc acc ir arg buf.
+  Tamarack n (mpc,mem,mar,pc,acc,ir,arg,buf) /\
+  (mpc 0 = 0)
+  ==>
+  !t. mpc (TimeOfCycle n (mem,pc,acc) t) = 0``,
+
+REPEAT STRIP_TAC >>
+Induct_on `t` >> (
+  METIS_TAC [EVERY_INST_THM, TimeOfCycle_def]
+))
+
+
+val CORRECTNESS_THM = store_thm ("CORRECTNESS_THM",
+``!n mpc mem mar pc acc ir arg buf.
+  Tamarack n (mpc,mem,mar,pc,acc,ir,arg,buf) /\
+  (mpc 0 = 0)
+  ==>
+  let f = TimeOfCycle n (mem,pc,acc) in
+  Behaviour n (mem o f,pc o f,acc o f)``,
+
+SIMP_TAC std_ss [Behaviour_def, LET_DEF, TimeOfCycle_def, GSYM ADD1] >>
+METIS_TAC[ALWAYS_MPC_0_THM, EVERY_INST_THM]);
 
 
 val _ = export_theory ();
